Superposition_Calculus/Ground_Order.thy
@@ -1,0 +1,9 @@
+theory Ground_Order
+  imports Ground_Term_Order Term_Order_Lifting
+begin
+
+locale ground_order =
+  term.order: ground_term_order +
+  term_order_lifting
+
+end
