Superposition_Calculus/Ground_Term_Order.thy
@@ -1,0 +1,120 @@
+theory Ground_Term_Order
+  imports 
+    Ground_Term_Extra
+    Ground_Context
+    Term_Order_Notation
+    Restricted_Order
+    Transitive_Closure_Extra
+begin
+
+locale context_compatibility_iff =
+  fixes R
+  assumes
+    context_compatibility_iff [simp]: "\<And>c t t'. R c\<langle>t\<rangle>\<^sub>G c\<langle>t'\<rangle>\<^sub>G \<longleftrightarrow> R t t'"
+
+locale context_compatibility =
+  total_strict_order where less = less\<^sub>t
+  for less\<^sub>t :: "'f gterm \<Rightarrow> 'f gterm \<Rightarrow> bool" +
+  assumes
+    context_compatibility [simp]: "\<And>c t t'. less\<^sub>t t t' \<Longrightarrow> less\<^sub>t c\<langle>t\<rangle>\<^sub>G c\<langle>t'\<rangle>\<^sub>G"
+begin
+
+(* TODO: Already here with t or just from Ground_Order on?*)
+interpretation term_order_notation.
+
+sublocale context_compatibility_iff "(\<prec>\<^sub>t)"
+proof unfold_locales
+  fix c t t'
+  show "c\<langle>t\<rangle>\<^sub>G \<prec>\<^sub>t c\<langle>t'\<rangle>\<^sub>G \<longleftrightarrow> t \<prec>\<^sub>t t'"
+  proof(intro iffI)
+    assume less\<^sub>t_with_context: "c\<langle>t\<rangle>\<^sub>G \<prec>\<^sub>t c\<langle>t'\<rangle>\<^sub>G"
+
+    show "t \<prec>\<^sub>t t'"
+    proof(rule ccontr)
+      assume "\<not> t \<prec>\<^sub>t t'"
+      hence "t' \<preceq>\<^sub>t t"
+        by order
+
+      show False
+      proof(cases "t' = t")
+        case True
+
+        then have "c\<langle>t\<rangle>\<^sub>G = c\<langle>t'\<rangle>\<^sub>G"
+          by blast
+
+        then show False
+          using less\<^sub>t_with_context 
+          by order
+      next
+        case False
+
+        then have "t' \<prec>\<^sub>t t"
+          using \<open>t' \<preceq>\<^sub>t t\<close> 
+          by order
+
+        then have "c\<langle>t'\<rangle>\<^sub>G \<prec>\<^sub>t c\<langle>t\<rangle>\<^sub>G"
+          using context_compatibility 
+          by metis
+
+        then show ?thesis
+          using less\<^sub>t_with_context 
+          by order
+      qed
+    qed
+  next
+    show "t \<prec>\<^sub>t t' \<Longrightarrow> c\<langle>t\<rangle>\<^sub>G \<prec>\<^sub>t c\<langle>t'\<rangle>\<^sub>G"
+      using context_compatibility.
+  qed
+qed
+
+sublocale less_eq: context_compatibility_iff "(\<preceq>\<^sub>t)"
+  using context_compatibility not_le
+  by unfold_locales blast
+
+end
+
+locale subterm_property =
+  strict_order where less = less\<^sub>t
+  for less\<^sub>t :: "'f gterm \<Rightarrow> 'f gterm \<Rightarrow> bool" +
+  assumes
+    subterm_property [simp]: "\<And>t c. c \<noteq> \<box> \<Longrightarrow> less\<^sub>t t c\<langle>t\<rangle>\<^sub>G"
+begin
+
+interpretation term_order_notation.
+
+lemma less_eq_subterm_property: "t \<preceq>\<^sub>t c\<langle>t\<rangle>\<^sub>G"
+  using subterm_property
+  by (metis gctxt_ident_iff_eq_GHole reflclp_iff)
+
+end
+
+locale ground_term_order = 
+  wellfounded_strict_order less\<^sub>t + 
+  total_strict_order less\<^sub>t +
+  context_compatibility less\<^sub>t +
+  subterm_property less\<^sub>t 
+  for less\<^sub>t :: "'f gterm \<Rightarrow> 'f gterm \<Rightarrow> bool" 
+begin
+
+interpretation term_order_notation.
+
+(* TODO: Names *)
+lemma context_less_term_less_eq:
+  assumes 
+    "\<And>t. c\<langle>t\<rangle>\<^sub>G \<prec>\<^sub>t c'\<langle>t\<rangle>\<^sub>G"
+    "t \<preceq>\<^sub>t t'"
+  shows "c\<langle>t\<rangle>\<^sub>G \<prec>\<^sub>t c'\<langle>t'\<rangle>\<^sub>G"
+  using assms context_compatibility
+  by (metis reflclp_iff dual_order.strict_trans)
+
+lemma context_less_eq_term_less:
+  assumes 
+    "\<And>t. c\<langle>t\<rangle>\<^sub>G \<preceq>\<^sub>t c'\<langle>t\<rangle>\<^sub>G"
+    "t \<prec>\<^sub>t t'"
+  shows "c\<langle>t\<rangle>\<^sub>G \<prec>\<^sub>t c'\<langle>t'\<rangle>\<^sub>G"
+  using assms context_compatibility dual_order.strict_trans1 
+  by blast
+
+end
+
+end
