Superposition_Calculus/Maximal_Literal.thy
@@ -1,0 +1,49 @@
+theory Maximal_Literal
+  imports 
+    Clausal_Calculus_Extra
+    Min_Max_Least_Greatest_Multiset 
+    Restricted_Order
+begin
+
+locale maximal_literal = order: strict_order where less = less 
+for less :: "'t uprod literal \<Rightarrow> 't uprod literal \<Rightarrow> bool"
+begin
+
+abbreviation is_maximal :: "'t uprod literal \<Rightarrow> 't uprod clause \<Rightarrow> bool" where
+  "is_maximal l C \<equiv> order.is_maximal_in_mset C l"
+
+abbreviation is_strictly_maximal :: "'t uprod literal \<Rightarrow> 't uprod clause \<Rightarrow> bool" where
+  "is_strictly_maximal l C \<equiv> order.is_strictly_maximal_in_mset C l"
+
+lemmas is_maximal_def = order.is_maximal_in_mset_iff
+
+lemmas is_strictly_maximal_def = order.is_strictly_maximal_in_mset_iff
+
+lemmas is_maximal_if_is_strictly_maximal = order.is_maximal_in_mset_if_is_strictly_maximal_in_mset
+
+lemma maximal_in_clause:
+  assumes "is_maximal l C"
+  shows "l \<in># C"
+  using assms 
+  unfolding is_maximal_def
+  by(rule conjunct1)
+
+lemma strictly_maximal_in_clause:
+  assumes "is_strictly_maximal l C"
+  shows "l \<in># C"
+  using assms  
+  unfolding is_strictly_maximal_def
+  by(rule conjunct1)
+
+(* TODO: Names *)
+lemma is_maximal_empty [simp]: "is_maximal l C \<Longrightarrow> C \<noteq> {#}"  
+  using maximal_in_clause
+  by fastforce
+
+lemma is_strictly_maximal_empty [simp]: "is_strictly_maximal l C \<Longrightarrow> C \<noteq> {#}"
+  using strictly_maximal_in_clause
+  by fastforce
+
+end
+
+end
