Superposition_Calculus/Nonground_Order.thy
@@ -1,0 +1,305 @@
+theory Nonground_Order
+  imports
+    Nonground_Term_Order
+    Term_Order_Lifting
+    Nonground_Clause
+    Relation_Extra
+begin
+
+section \<open>Nonground Order\<close>
+
+locale nonground_order_lifting = 
+  total_grounded_multiset_extension +
+  ground_subst_stable_total_multiset_extension +
+  subst_update_stable_multiset_extension
+begin
+
+sublocale grounded_restricted_total_strict_order where
+  less = multiset_extension and subst = "subst" and vars = vars and to_ground = to_ground and 
+  from_ground = "from_ground"
+  by unfold_locales
+
+end
+
+locale nonground_term_based_order_lifting = nonground_order_lifting where 
+  id_subst = Var and comp_subst = "(\<odot>)" and base_vars = term.vars and base_less = less\<^sub>t and 
+  base_subst = "(\<cdot>t)"
+for less\<^sub>t
+
+locale nonground_order =
+  restricted_term_order_lifting where
+  restriction = "range term.from_ground" and
+  less\<^sub>t = "less\<^sub>t :: ('f, 'v) Term.term \<Rightarrow> ('f, 'v) Term.term \<Rightarrow> bool" +
+  term.order: nonground_term_order
+begin
+
+(* TODO: Find way to not have this twice *)
+notation term.order.less\<^sub>G (infix "\<prec>\<^sub>t\<^sub>G" 50)
+notation term.order.less_eq\<^sub>G (infix "\<preceq>\<^sub>t\<^sub>G" 50)
+
+sublocale literal.order: nonground_term_based_order_lifting where 
+  less = less\<^sub>t and sub_subst = "(\<cdot>t)" and sub_vars = term.vars and sub_to_ground = term.to_ground and 
+  sub_from_ground = term.from_ground and map = map_literal_term and to_set = literal_to_term_set and
+  to_ground_map = map_literal_term and from_ground_map = map_literal_term and 
+  ground_map = map_literal_term and to_set_ground = literal_to_term_set and to_mset = mset_lit
+rewrites
+  "\<And>l \<sigma>. functional_substitution_lifting.subst (\<cdot>t) map_literal_term l \<sigma> = literal.subst l \<sigma>" and
+  "\<And>l. functional_substitution_lifting.vars term.vars literal_to_term_set l = literal.vars l" and
+  "\<And>l\<^sub>G. grounding_lifting.from_ground term.from_ground map_literal_term l\<^sub>G = 
+    literal.from_ground l\<^sub>G" and
+  "\<And>l. grounding_lifting.to_ground term.to_ground map_literal_term l = literal.to_ground l"
+  by unfold_locales (auto simp: inj_mset_lit mset_lit_image_mset)
+
+notation literal.order.less\<^sub>G (infix "\<prec>\<^sub>l\<^sub>G" 50)
+notation literal.order.less_eq\<^sub>G (infix "\<preceq>\<^sub>l\<^sub>G" 50)
+
+sublocale literal.order.restriction: maximal_literal "(\<prec>\<^sub>l\<^sub>G)"
+  by unfold_locales
+
+sublocale clause.order: nonground_term_based_order_lifting where 
+  less = "(\<prec>\<^sub>l)" and sub_subst = literal.subst and sub_vars = literal.vars and
+  sub_to_ground = literal.to_ground and sub_from_ground = literal.from_ground and 
+  map = image_mset and to_set = set_mset and to_ground_map = image_mset and 
+  from_ground_map = image_mset and ground_map = image_mset and 
+  to_set_ground = set_mset and to_mset = "\<lambda>x. x"
+  by unfold_locales simp_all
+ 
+notation clause.order.less\<^sub>G (infix "\<prec>\<^sub>c\<^sub>G" 50)
+notation clause.order.less_eq\<^sub>G (infix "\<preceq>\<^sub>c\<^sub>G" 50)
+
+lemma obtain_maximal_literal: (* is_maximal_ground_subst_stability *)
+  assumes 
+    not_empty: "C \<noteq> {#}" and
+    grounding: "clause.is_ground (C \<cdot> \<gamma>)" 
+  obtains l
+  where "is_maximal l C" "is_maximal (l \<cdot>l \<gamma>) (C \<cdot> \<gamma>)"
+proof-
+
+  have grounding_not_empty: "C \<cdot> \<gamma> \<noteq> {#}"
+    using not_empty clause_subst_empty(2) 
+    by blast
+    
+  obtain l where 
+    l_in_C: "l \<in># C" and
+    l_grounding_is_maximal: "is_maximal (l \<cdot>l \<gamma>) (C \<cdot> \<gamma>)" 
+    using
+      ex_maximal_in_mset_wrt[OF 
+        literal.order.transp_on_less literal.order.asymp_on_less grounding_not_empty]  
+      maximal_in_clause
+    unfolding clause.subst_def
+    by (metis (mono_tags, lifting) image_iff multiset.set_map)
+
+  show ?thesis
+  proof(cases "is_maximal l C")
+    case True
+
+    with l_grounding_is_maximal that 
+    show ?thesis
+      by blast
+  next
+    case False
+    then obtain l' where 
+      l'_in_C: "l' \<in># C" and 
+      l_less_l': "l \<prec>\<^sub>l l'" 
+      unfolding is_maximal_def
+      using l_in_C
+      by blast 
+
+    note literals_in_C = l_in_C l'_in_C
+    note literals_grounding = literals_in_C[THEN clause.to_set_is_ground_subst[OF _ grounding]]
+
+    have "l \<cdot>l \<gamma> \<prec>\<^sub>l l' \<cdot>l \<gamma>"
+      using literal.order.ground_subst_stability[OF literals_grounding l_less_l'].
+   
+    then have False
+     using 
+       l_grounding_is_maximal
+       clause.subst_in_to_set_subst[OF l'_in_C] 
+     unfolding is_maximal_def
+     by force
+       
+    then show ?thesis..
+  qed
+qed
+
+lemma obtain_strictly_maximal_literal: (* is_strictly_maximal\<^sub>l_ground_subst_stability *)
+  assumes 
+   grounding: "clause.is_ground (C \<cdot> \<gamma>)" and
+   ground_strictly_maximal: "is_strictly_maximal l\<^sub>G (C \<cdot> \<gamma>)"
+ obtains l where 
+   "is_strictly_maximal l C" "l\<^sub>G = l \<cdot>l \<gamma>"
+proof-
+ 
+  have grounding_not_empty: "C \<cdot> \<gamma> \<noteq> {#}"
+    using ground_strictly_maximal
+    by simp
+
+  have l\<^sub>G_in_grounding: "l\<^sub>G \<in># C \<cdot> \<gamma>"
+    using strictly_maximal_in_clause[OF ground_strictly_maximal].
+   
+  obtain l where 
+    l_in_C: "l \<in># C" and 
+    grounded_l [simp]: "l\<^sub>G = l \<cdot>l \<gamma>"
+    using l\<^sub>G_in_grounding 
+    unfolding clause.subst_def
+    by blast
+
+  show ?thesis
+  proof(cases "is_strictly_maximal l C")
+    case True
+    show ?thesis
+      using that[OF True grounded_l].
+  next
+    case False
+
+    then obtain l' where
+      l'_in_C: "l' \<in># C - {# l #}" and
+      l_less_eq_l': "l \<preceq>\<^sub>l l'" 
+      unfolding is_strictly_maximal_def
+      using l_in_C 
+      by blast
+      
+    note l_grounding = 
+       clause.to_set_is_ground_subst[OF l_in_C grounding]
+
+    have l'_grounding: "literal.is_ground (l' \<cdot>l \<gamma>)"
+      using l'_in_C grounding
+      by (meson clause.to_set_is_ground_subst in_diffD)
+
+    have "l \<cdot>l \<gamma> \<preceq>\<^sub>l l' \<cdot>l \<gamma>"
+      using literal.order.less_eq.ground_subst_stability[OF l_grounding l'_grounding l_less_eq_l'].
+
+    then have False
+      using clause.subst_in_to_set_subst[OF l'_in_C] ground_strictly_maximal 
+      unfolding is_strictly_maximal_def subst_clause_remove1_mset[OF l_in_C]
+      by simp
+   
+    then show ?thesis..
+  qed
+qed
+
+lemma is_maximal_if_grounding_is_maximal: (* is_maximal\<^sub>l_ground_subst_stability' *)
+  assumes 
+   l_in_C: "l \<in># C" and
+   C_grounding: "clause.is_ground (C \<cdot> \<gamma>)" and
+   l_grounding_is_maximal: "is_maximal (l \<cdot>l \<gamma>) (C \<cdot> \<gamma>)"
+ shows 
+   "is_maximal l C"
+proof(rule ccontr)
+  assume "\<not> is_maximal l C"
+
+  then obtain l' where l_less_l': "l \<prec>\<^sub>l l'" and l'_in_C: "l' \<in># C"
+    using l_in_C
+    unfolding is_maximal_def
+    by blast
+
+  have l'_grounding: "literal.is_ground (l' \<cdot>l \<gamma>)"
+    using clause.to_set_is_ground_subst[OF l'_in_C C_grounding].
+
+  have l_grounding: "literal.is_ground (l \<cdot>l \<gamma>)"
+    using clause.to_set_is_ground_subst[OF l_in_C C_grounding].
+
+  have l_grounding_in_C_grounding: "l' \<cdot>l \<gamma> \<in># C \<cdot> \<gamma>"
+    using clause.subst_in_to_set_subst[OF l'_in_C].
+     
+  have "l \<cdot>l \<gamma> \<prec>\<^sub>l l' \<cdot>l \<gamma>"
+    using literal.order.ground_subst_stability[OF l_grounding l'_grounding l_less_l'].
+  
+  then have "\<not> is_maximal (l \<cdot>l \<gamma>) (C \<cdot> \<gamma>)"
+    using l_grounding_in_C_grounding 
+    unfolding is_maximal_def literal.subst_comp_subst
+    by fastforce
+  
+  then show False
+    using l_grounding_is_maximal..
+qed
+
+lemma is_strictly_maximal_if_grounding_is_strictly_maximal: (* is_strictly_maximal\<^sub>l_ground_subst_stability' *)
+  assumes 
+   l_in_C: "l \<in># C" and
+   grounding: "clause.is_ground (C \<cdot> \<gamma>)" and
+   grounding_strictly_maximal: "is_strictly_maximal (l \<cdot>l \<gamma>) (C \<cdot> \<gamma>)"
+ shows 
+   "is_strictly_maximal l C"
+  using
+    is_maximal_if_grounding_is_maximal[OF 
+      l_in_C
+      grounding
+      is_maximal_if_is_strictly_maximal[OF grounding_strictly_maximal]
+    ]
+    grounding_strictly_maximal  
+  unfolding 
+    is_strictly_maximal_def is_maximal_def
+    subst_clause_remove1_mset[OF l_in_C, symmetric]
+    reflclp_iff
+  by (metis in_diffD clause.subst_in_to_set_subst)
+
+lemma unique_maximal_in_ground_clause:
+  assumes
+    "clause.is_ground C" 
+    "is_maximal l C"
+    "is_maximal l' C"
+  shows
+    "l = l'"
+  using assms clause.to_set_is_ground literal.order.not_less_eq 
+  unfolding is_maximal_def reflclp_iff
+  by meson
+
+lemma unique_strictly_maximal_in_ground_clause:
+  assumes
+    "clause.is_ground C" 
+    "is_strictly_maximal l C"
+    "is_strictly_maximal l' C"
+  shows
+    "l = l'"
+  using assms unique_maximal_in_ground_clause 
+  by blast
+
+
+
+
+(* TODO: Put in right sections + naming *)
+
+lemma less\<^sub>t_less\<^sub>l: 
+  assumes "term\<^sub>1 \<prec>\<^sub>t term\<^sub>2"
+  shows 
+    less\<^sub>t_less\<^sub>l_pos: "term\<^sub>1 \<approx> term\<^sub>3 \<prec>\<^sub>l term\<^sub>2 \<approx> term\<^sub>3" and
+    less\<^sub>t_less\<^sub>l_neg: "term\<^sub>1 !\<approx> term\<^sub>3 \<prec>\<^sub>l term\<^sub>2 !\<approx> term\<^sub>3"
+  using assms
+  unfolding less\<^sub>l_def
+  by (auto simp: multp_add_mset multp_add_mset' multp_add_same)
+
+lemma literal_order_all_less_eq_ex_less_set:
+  assumes 
+    "\<forall>term \<in> set_uprod (atm_of literal). term \<cdot>t \<sigma>' \<preceq>\<^sub>t term \<cdot>t \<sigma>"
+    "\<exists>term \<in> set_uprod (atm_of literal). term \<cdot>t \<sigma>' \<prec>\<^sub>t term \<cdot>t \<sigma>"
+  shows "literal \<cdot>l \<sigma>' \<prec>\<^sub>l literal \<cdot>l \<sigma>"
+  using literal.order.all_less_eq_ex_less[OF assms[folded set_mset_set_uprod]].
+ 
+lemma less\<^sub>c_add_mset:
+  assumes "l \<prec>\<^sub>l l'" "C \<preceq>\<^sub>c C'"
+  shows "add_mset l C \<prec>\<^sub>c add_mset l' C'"
+  using assms multp_add_mset_reflclp[OF literal.order.asymp literal.order.transp]
+  unfolding less\<^sub>c_def
+  by blast
+
+lemmas less\<^sub>c_add_same =
+  multp_add_same[OF literal.order.asymp literal.order.transp, folded less\<^sub>c_def]
+
+(* TODO: Scope *)
+lemma less_eq\<^sub>l_less_eq\<^sub>c:
+  assumes "\<forall>literal \<in># clause. literal \<cdot>l \<sigma>' \<preceq>\<^sub>l literal \<cdot>l \<sigma>"
+  shows "clause \<cdot> \<sigma>' \<preceq>\<^sub>c clause \<cdot> \<sigma>"
+  using clause.order.all_less_eq[OF assms]. 
+ 
+lemma less\<^sub>l_less\<^sub>c:
+  assumes 
+    "\<forall>literal \<in># clause. literal \<cdot>l \<sigma>' \<preceq>\<^sub>l literal \<cdot>l \<sigma>"
+    "\<exists>literal \<in># clause. literal \<cdot>l \<sigma>' \<prec>\<^sub>l literal \<cdot>l \<sigma>"
+  shows "clause \<cdot> \<sigma>' \<prec>\<^sub>c clause \<cdot> \<sigma>"
+  using clause.order.all_less_eq_ex_less[OF assms].
+
+
+end
+
+end
