Superposition_Calculus/Nonground_Term.thy
@@ -21,6 +21,7 @@ section \<open>Nonground Terms and Substitutions\<close>
 type_synonym 'f ground_term = "'f gterm"
 type_synonym ('f, 'v) "context" = "('f, 'v) ctxt"
 
+(* TODO: Already here with t or just from Nonground_Clause on?*)
 notation subst_apply_term (infixl "\<cdot>t" 67)
 notation subst_compose (infixl "\<odot>" 75)
 
@@ -103,7 +104,8 @@ next
     by auto
 qed
 
-locale "term" = 
+(* TODO: Name *)
+locale term_sth = 
   base_functional_substitution +
   finite_variables +
   all_subst_ident_iff_ground + 
@@ -114,7 +116,7 @@ locale term_grounding =
   variables_in_base_imgu where base_vars = vars and base_subst = subst +
   grounding
 
-global_interpretation "term": "term" where subst = "(\<cdot>t)" and  id_subst = Var and 
+global_interpretation "term": term_sth where subst = "(\<cdot>t)" and  id_subst = Var and 
   comp_subst = "(\<odot>)" and
    vars = "term.vars :: ('f, 'v) term \<Rightarrow> 'v set"  and subst_domain = subst_domain and 
    range_vars = range_vars
@@ -257,134 +259,6 @@ lemma renaming_surj_the_inv:
   using assms the_inv_f_f
   unfolding term_subst_is_renaming_iff is_Var_def surj_def
   by metis
-
-subsection \<open>Entailment\<close>
-
-lemma var_in_term:
-  assumes "x \<in> term.vars t"
-  obtains c where "t = c\<langle>Var x\<rangle>"
-  using assms
-proof(induction t)
-  case Var
-  then show ?case
-    by (meson supteq_Var supteq_ctxtE)
-next
-  case (Fun f args)
-  then obtain t' where "t' \<in> set args " "x \<in> term.vars t'"
-    by (metis term.distinct(1) term.sel(4) term.set_cases(2))
-
-  moreover then obtain args1 args2 where
-    "args1 @ [t'] @ args2 = args"
-    by (metis append_Cons append_Nil split_list)
-
-  moreover then have "(More f args1 \<box> args2)\<langle>t'\<rangle> = Fun f args"
-    by simp
-
-  ultimately show ?case 
-    using Fun(1)
-    by (meson assms supteq_ctxtE that vars_term_supteq)
-qed
-
-lemma vars_term_ms_count:
-  assumes "term.is_ground t"
-  shows 
-    "size {#x' \<in># vars_term_ms c\<langle>Var x\<rangle>. x' = x#} = Suc (size {#x' \<in># vars_term_ms c\<langle>t\<rangle>. x' = x#})"
-  by(induction c)(auto simp: assms filter_mset_empty_conv)
-
-locale term_entailment =
-  fixes I :: "('f gterm \<times> 'f gterm) set"
-  assumes 
-    trans: "trans I" and
-    sym: "sym I" and
-    compatible_with_gctxt: "compatible_with_gctxt I"
-begin
-
-lemma symmetric_context_congruence:
-  assumes "(t, t') \<in> I"
-  shows "(c\<langle>t\<rangle>\<^sub>G, t'') \<in> I \<longleftrightarrow> (c\<langle>t'\<rangle>\<^sub>G, t'') \<in> I"
-  by (meson assms compatible_with_gctxt compatible_with_gctxtD sym trans symD transE)
-
-sublocale "term": symmetric_base_entailment where 
-  vars = "term.vars :: ('f, 'v) term \<Rightarrow> 'v set" and id_subst = Var and comp_subst = "(\<odot>)" and 
-  subst = "(\<cdot>t)" and to_ground = term.to_ground and from_ground = term.from_ground
-proof unfold_locales
-  fix \<gamma> :: "('f, 'v) subst" and t t' update var
-
-  assume 
-    update_is_ground: "term.is_ground update" and
-    var_grounding: "term.is_ground (\<gamma> var)" and
-    var_update: "(term.to_ground (\<gamma> var), term.to_ground update) \<in> I" and
-    term_grounding: "term.is_ground (t \<cdot>t \<gamma>)" and
-    updated_term: "(term.to_ground (t \<cdot>t \<gamma>(var := update)), t') \<in> I"
-
-  from term_grounding updated_term
-  show "(term.to_ground (t \<cdot>t \<gamma>), t') \<in> I"
-  proof(induction "size (filter_mset (\<lambda>var'. var' = var) (vars_term_ms t))" arbitrary: t)
-    case 0
-
-    then have "var \<notin> term.vars t"
-      by (metis (mono_tags, lifting) filter_mset_empty_conv set_mset_vars_term_ms 
-          size_eq_0_iff_empty)
-
-    then have "t \<cdot>t \<gamma>(var := update) = t \<cdot>t \<gamma>"
-      using term.subst_reduntant_upd 
-      by (simp add: eval_with_fresh_var)
-
-    with 0 show ?case
-      by argo
-  next
-    case (Suc n)
-
-    let ?context_to_ground = "map_args_actxt term.to_ground"
-
-    have "var \<in> term.vars t"
-      using Suc.hyps(2)
-      by (metis (full_types) filter_mset_empty_conv nonempty_has_size set_mset_vars_term_ms 
-          zero_less_Suc)
-
-    then obtain c where t [simp]: "t = c\<langle>Var var\<rangle>"
-      by (meson var_in_term)
-
-    have [simp]: 
-      "(?context_to_ground (c \<cdot>t\<^sub>c \<gamma>))\<langle>term.to_ground (\<gamma> var)\<rangle>\<^sub>G = term.to_ground (c\<langle>Var var\<rangle> \<cdot>t \<gamma>)"
-      using Suc 
-      by(induction c) simp_all
-
-    have context_update [simp]: 
-      "(?context_to_ground (c \<cdot>t\<^sub>c \<gamma>))\<langle>term.to_ground update\<rangle>\<^sub>G = term.to_ground (c\<langle>update\<rangle> \<cdot>t \<gamma>)"
-      using Suc update_is_ground
-      by(induction c) auto
-
-    have "n = size {#var' \<in># vars_term_ms c\<langle>update\<rangle>. var' = var#}"
-      using Suc vars_term_ms_count[OF update_is_ground, of var c]
-      by auto
-
-    moreover have "term.is_ground (c\<langle>update\<rangle> \<cdot>t \<gamma>)"
-      using Suc.prems update_is_ground 
-      by auto
-
-    moreover have "(term.to_ground (c\<langle>update\<rangle> \<cdot>t \<gamma>(var := update)), t') \<in> I"
-      using Suc.prems update_is_ground
-      by auto
-
-    moreover have "(term.to_ground update, term.to_ground (\<gamma> var)) \<in> I"
-      using var_update sym
-      by (metis symD)
-
-    moreover have "(term.to_ground (c\<langle>update\<rangle> \<cdot>t \<gamma>), t') \<in> I"
-      using Suc calculation
-      by blast
-
-    ultimately have "((?context_to_ground (c \<cdot>t\<^sub>c \<gamma>))\<langle>term.to_ground (\<gamma> var)\<rangle>\<^sub>G, t') \<in> I"
-      using symmetric_context_congruence context_update
-      by metis
-
-    then show ?case 
-      by simp
-  qed
-qed (rule sym)
-
-end
 
 subsection\<open>Setup for lifting from terms\<close>
 
