Superposition_Calculus/Nonground_Term_Order.thy
@@ -1,0 +1,238 @@
+theory Nonground_Term_Order
+  imports
+    Nonground_Term
+    Nonground_Context
+    Ground_Order
+begin
+
+locale ground_context_compatibility =
+  fixes R
+  assumes ground_context_compatibility: 
+    "\<And>c t\<^sub>1 t\<^sub>2. 
+      R t\<^sub>1 t\<^sub>2 \<Longrightarrow>
+      term.is_ground t\<^sub>1 \<Longrightarrow>
+      term.is_ground t\<^sub>2 \<Longrightarrow>
+      context.is_ground c \<Longrightarrow>
+      R c\<langle>t\<^sub>1\<rangle> c\<langle>t\<^sub>2\<rangle>"
+
+locale ground_subterm_property =
+  fixes R
+  assumes ground_subterm_property: 
+    "\<And>t\<^sub>G c\<^sub>G. 
+      term.is_ground t\<^sub>G \<Longrightarrow>
+      context.is_ground c\<^sub>G \<Longrightarrow>
+      c\<^sub>G \<noteq> \<box> \<Longrightarrow>
+      R t\<^sub>G c\<^sub>G\<langle>t\<^sub>G\<rangle>"
+
+locale grounded_term_order = 
+  subst_update_stable_grounded_order where 
+  less = less\<^sub>t and base_less = less\<^sub>t and base_subst = subst and base_vars = vars +
+  grounded_restricted_total_strict_order where less = less\<^sub>t +
+  grounded_restricted_wellfounded_strict_order where less = less\<^sub>t +
+  ground_subst_stable_grounded_order where less = less\<^sub>t
+for less\<^sub>t
+
+locale nonground_term_order = 
+  restricted_wellfounded_total_strict_order where 
+  less = less\<^sub>t and restriction = "range term.from_ground" +
+  ground_subst_stability where R = less\<^sub>t and comp_subst = "(\<odot>)" and subst = "(\<cdot>t)" and 
+  vars = term.vars and id_subst = Var and to_ground = term.to_ground and 
+  from_ground = "term.from_ground" + 
+  ground_context_compatibility where R = less\<^sub>t  +
+  ground_subterm_property where R = less\<^sub>t
+for less\<^sub>t :: "('f, 'v) Term.term \<Rightarrow> ('f, 'v) Term.term \<Rightarrow> bool"
+begin
+
+(* TODO: Already here with t or just from Nonground_Order on? *)
+interpretation term_order_notation.
+
+sublocale grounded_term_order where (* TODO! Scope *)
+  comp_subst = "(\<odot>)" and subst = "(\<cdot>t)" and vars = term.vars and id_subst = Var and 
+  to_ground = term.to_ground and from_ground = "term.from_ground"
+proof unfold_locales
+  fix update x \<gamma> and t :: "('f, 'v) term"
+  assume 
+    update_is_ground: "term.is_ground update" and 
+    update_less: "update \<prec>\<^sub>t \<gamma> x" and 
+    term_grounding: "term.is_ground (t \<cdot>t \<gamma>)" and
+    var: "x \<in> term.vars t"
+
+  from term_grounding var 
+  show "t \<cdot>t \<gamma>(x := update) \<prec>\<^sub>t t \<cdot>t \<gamma>" 
+  proof(induction t)
+    case Var
+    then show ?case 
+      using update_is_ground update_less
+      by simp
+  next
+    case (Fun f subs)
+
+    then have "\<forall>sub \<in> set subs. sub \<cdot>t \<gamma>(x := update) \<preceq>\<^sub>t sub \<cdot>t \<gamma>"
+      by (metis eval_with_fresh_var is_ground_iff reflclp_iff term.set_intros(4))
+
+    moreover then have "\<exists>sub \<in> set subs. sub \<cdot>t \<gamma>(x := update) \<prec>\<^sub>t sub \<cdot>t \<gamma>"
+      using Fun update_less
+      by (metis (full_types) fun_upd_same term.distinct(1) term.sel(4) term.set_cases(2)
+          dual_order.strict_iff_order term_subst_eq_rev)
+
+    ultimately show ?case
+      using Fun(2, 3)
+    proof(induction "filter (\<lambda>sub. sub \<cdot>t \<gamma>(x := update) \<prec>\<^sub>t sub \<cdot>t \<gamma>) subs" arbitrary: subs)
+      case Nil
+      then show ?case
+        unfolding empty_filter_conv
+        by blast
+    next
+      case first: (Cons s ss)
+
+      have update_grounding [simp]: "term.is_ground (s \<cdot>t \<gamma>(x := update))"
+        using first.prems(3) update_is_ground first.hyps(2)
+        by (metis (no_types, lifting) filter_eq_ConsD fun_upd_other fun_upd_same in_set_conv_decomp 
+            is_ground_iff term.set_intros(4))
+
+      then have t_grounding [simp]: "term.is_ground (s \<cdot>t \<gamma>)"
+        using update_grounding Fun.prems(1,2)
+        by (metis fun_upd_other is_ground_iff)
+
+      show ?case
+      proof(cases ss)
+        case Nil
+        then obtain ss1 ss2 where subs: "subs = ss1 @ s # ss2"
+          using filter_eq_ConsD[OF first.hyps(2)[symmetric]]
+          by blast
+
+        have ss1: "\<forall>s \<in> set ss1. s \<cdot>t \<gamma>(x := update) = s \<cdot>t \<gamma>"
+          using first.hyps(2) first.prems(1) 
+          unfolding Nil subs
+          by (smt (verit, del_insts) Un_iff append_Cons_eq_iff filter_empty_conv filter_eq_ConsD 
+              set_append antisym_conv2)
+
+        have ss2: "\<forall>s \<in> set ss2. s \<cdot>t \<gamma>(x := update) = s \<cdot>t \<gamma>"
+          using first.hyps(2) first.prems(1) 
+          unfolding Nil subs
+          by (smt (verit, ccfv_SIG) Un_iff append_Cons_eq_iff filter_empty_conv filter_eq_ConsD 
+              list.set_intros(2) set_append antisym_conv2)
+
+        let ?c = "More f (map (\<lambda>s. s \<cdot>t \<gamma>) ss1) \<box> (map (\<lambda>s. s \<cdot>t \<gamma>) ss2)"
+
+        have "term.is_ground (s \<cdot>t \<gamma>)"
+          using subs first(5)
+          by auto
+
+        moreover then have "term.is_ground (s \<cdot>t \<gamma>(x := update))"
+          by (metis update_is_ground fun_upd_other fun_upd_same is_ground_iff)
+
+        moreover have "context.is_ground ?c"
+          using subs first(5)
+          by auto
+
+        moreover have "s \<cdot>t \<gamma>(x := update) \<prec>\<^sub>t s \<cdot>t \<gamma>" 
+          using first.hyps(2)
+          by (meson Cons_eq_filterD)
+
+        ultimately have "?c\<langle>s \<cdot>t \<gamma>(x := update)\<rangle> \<prec>\<^sub>t ?c\<langle>s \<cdot>t \<gamma>\<rangle>"
+          using ground_context_compatibility
+          by blast
+
+        moreover have "Fun f subs \<cdot>t \<gamma>(x := update) = ?c\<langle>s \<cdot>t \<gamma>(x := update)\<rangle>"
+          unfolding subs
+          using ss1 ss2
+          by simp
+
+        moreover have "Fun f subs \<cdot>t \<gamma> = ?c\<langle>s \<cdot>t \<gamma>\<rangle>"
+          unfolding subs
+          by auto
+
+        ultimately show ?thesis
+          by argo
+      next
+        case (Cons t' ts')
+
+        from first(2)
+        obtain ss1 ss2 where
+          subs: "subs = ss1 @ s # ss2" and
+          ss1: "\<forall>s\<in>set ss1. \<not> s \<cdot>t \<gamma>(x := update) \<prec>\<^sub>t s \<cdot>t \<gamma>" and
+          less: "s \<cdot>t \<gamma>(x := update) \<prec>\<^sub>t s \<cdot>t \<gamma>" and 
+          ss: "ss = filter (\<lambda>term. term \<cdot>t \<gamma>(x := update)\<prec>\<^sub>t term \<cdot>t \<gamma>) ss2"
+          using Cons_eq_filter_iff[of s ss "(\<lambda>s. s \<cdot>t \<gamma>(x := update) \<prec>\<^sub>t s \<cdot>t \<gamma>)"]
+          by blast
+
+        let ?subs' = "ss1 @ (s \<cdot>t \<gamma>(x := update)) # ss2"
+
+        have [simp]: "s \<cdot>t \<gamma>(x := update) \<cdot>t \<gamma> = s \<cdot>t \<gamma>(x := update)"
+          using first.prems(3) update_is_ground
+          unfolding subs
+          by (simp add: is_ground_iff)
+
+        have [simp]: "s \<cdot>t \<gamma>(x := update) \<cdot>t \<gamma>(x := update) = s \<cdot>t \<gamma>(x := update)"
+          using first.prems(3) update_is_ground
+          unfolding subs
+          by (simp add: is_ground_iff)
+
+        have ss: "ss = filter (\<lambda>sub. sub \<cdot>t \<gamma>(x := update) \<prec>\<^sub>t sub \<cdot>t \<gamma>) ?subs'" 
+          using ss1 ss
+          by auto
+
+        moreover have "\<forall>sub \<in> set ?subs'. sub \<cdot>t \<gamma>(x := update) \<preceq>\<^sub>t sub \<cdot>t \<gamma>"
+          using first.prems(1)
+          unfolding subs
+          by simp
+
+        moreover have ex_less: "\<exists>sub \<in> set ?subs'. sub \<cdot>t \<gamma>(x := update) \<prec>\<^sub>t sub \<cdot>t \<gamma>"
+          using ss Cons neq_Nil_conv by force
+
+        moreover have subs'_grounding: "term.is_ground (Fun f ?subs' \<cdot>t \<gamma>)"
+          using first.prems(3)
+          unfolding subs
+          by simp
+
+        moreover have "x \<in> term.vars (Fun f ?subs')"
+          by (metis ex_less eval_with_fresh_var term.set_intros(4) less_irrefl)
+
+        ultimately have less_subs': "Fun f ?subs' \<cdot>t \<gamma>(x := update) \<prec>\<^sub>t Fun f ?subs' \<cdot>t \<gamma>"
+          using first.hyps(1) first.prems(3) by blast
+
+        have context_grounding: "context.is_ground (More f ss1 \<box> ss2 \<cdot>t\<^sub>c \<gamma>)"
+          using subs'_grounding
+          by auto
+
+        have "Fun f (ss1 @ s \<cdot>t \<gamma>(x := update) # ss2) \<cdot>t \<gamma> \<prec>\<^sub>t Fun f subs \<cdot>t \<gamma>"
+          unfolding subs
+          using ground_context_compatibility[OF less _ _ context_grounding]
+          by simp
+
+        with less_subs' show ?thesis 
+          unfolding subs
+          by simp
+      qed
+    qed
+  qed
+qed
+
+(* TODO: Find way to not have this twice \<longrightarrow> Use here just with G when up the t are also removed *)
+notation less\<^sub>G (infix "\<prec>\<^sub>t\<^sub>G" 50)
+notation less_eq\<^sub>G (infix "\<preceq>\<^sub>t\<^sub>G" 50)
+
+sublocale restriction: ground_term_order "(\<prec>\<^sub>t\<^sub>G)"
+proof unfold_locales
+  fix c t t'
+  assume "t \<prec>\<^sub>t\<^sub>G t'"
+  then show "c\<langle>t\<rangle>\<^sub>G \<prec>\<^sub>t\<^sub>G c\<langle>t'\<rangle>\<^sub>G"
+    using ground_context_compatibility[OF _ 
+        term.ground_is_ground term.ground_is_ground context.ground_is_ground]
+    unfolding less\<^sub>G_def ground_term_with_context(3)
+    by simp
+next
+  fix t :: "'f gterm" and c :: "'f ground_context"
+  assume "c \<noteq> \<box>"
+  then show "t \<prec>\<^sub>t\<^sub>G c\<langle>t\<rangle>\<^sub>G"
+    using 
+      ground_subterm_property[OF term.ground_is_ground context.ground_is_ground]
+      context_from_ground_hole
+    unfolding ground_term_with_context(3) less\<^sub>G_def
+    by blast
+qed
+
+end
+
+end
