Superposition_Calculus/Term_Order_Lifting.thy
@@ -1,0 +1,58 @@
+theory Term_Order_Lifting
+  imports 
+    Grounded_Multiset_Extension
+    Maximal_Literal
+    Term_Order_Notation
+begin
+
+locale restricted_term_order_lifting =
+  term.order: restricted_wellfounded_total_strict_order where less = less\<^sub>t
+for less\<^sub>t
+begin
+
+sublocale term_order_notation.
+
+abbreviation literal_order_restriction where
+  "literal_order_restriction \<equiv> {b. set_mset (mset_lit b) \<subseteq> restriction}"
+
+sublocale literal.order: restricted_total_multiset_extension where 
+  less = "(\<prec>\<^sub>t)" and to_mset = mset_lit
+  using inj_mset_lit
+  by unfold_locales (auto simp: inj_on_def)
+
+notation literal.order.multiset_extension (infix "\<prec>\<^sub>l" 50)
+notation literal.order.less_eq (infix "\<preceq>\<^sub>l" 50)
+
+lemmas less\<^sub>l_def = literal.order.multiset_extension_def
+
+sublocale maximal_literal "(\<prec>\<^sub>l)"
+  by unfold_locales
+
+sublocale clause.order: restricted_total_multiset_extension where 
+  less = "(\<prec>\<^sub>l)" and to_mset = "\<lambda>x. x" and restriction = literal_order_restriction
+  by unfold_locales auto
+
+notation clause.order.multiset_extension (infix "\<prec>\<^sub>c" 50) 
+notation clause.order.less_eq (infix "\<preceq>\<^sub>c" 50)
+
+lemmas less\<^sub>c_def = clause.order.multiset_extension_def
+
+end
+
+locale term_order_lifting =  
+  restricted_term_order_lifting where restriction = UNIV +
+  term.order: wellfounded_strict_order less\<^sub>t + 
+  term.order: total_strict_order less\<^sub>t
+begin
+
+sublocale literal.order: total_wellfounded_multiset_extension where 
+  less = "(\<prec>\<^sub>t)" and to_mset = mset_lit
+  by unfold_locales (simp add: inj_mset_lit)
+
+sublocale clause.order: total_wellfounded_multiset_extension where 
+  less = "(\<prec>\<^sub>l)"  and to_mset = "\<lambda>x. x" 
+  by unfold_locales simp
+
+end
+
+end
